\section*{H8 i)}

\subsection*{Behauptung}

$ \frac{1-x}{1+x} = 1 + 2 \sum\limits_{\nu=1}^{\infty} (-1)^{\nu} x^{\nu}$, f端r $x \in (-1,1) $

\subsection*{Beweis}

\subsubsection*{Behauptung}

F端r $n \in \mathbb{N}_{>0}$ gilt:

$(-1-x)\sum\limits^{n}_{\nu=1}(-1)^{\nu}x^{\nu} = x+(-1)^{(n+1)}x^{(n+1)}$

\subsubsection*{Beweis}

\paragraph*{IA}

F端r $n = 1$ gilt:


$(-1-x)\sum\limits^{1}_{\nu=1}(-1)^{\nu}x^{\nu} =(-1-x)-x= x+x^{2}$

\paragraph*{IV}

Sei $n \in \mathbb{N}_{>0}$ mit 
$(-1-x)\sum\limits^{n}_{\nu=1}(-1)^{\nu}x^{\nu} = x+(-1)^{(n+1)}x^{(n+1)}$

\paragraph*{IS}

$  (-1-x)\sum\limits^{n+1}_{\nu=1}(-1)^{\nu}x^{\nu} $

$ = (-1-x)\sum\limits^{n}_{\nu = 1}(-1)^{\nu} x^{\nu} + (-1-x) (-1)^{(n+1)} x^{(n+1)} $

$ \overset{IV}{=} x + (-1)^{(n+1)} n^{(n+1)} + (-1-x) (-1)^{(n+1)} x^{(n+1)}$

$ =  x + (-1)^{(n+1)} n^{(n+1)} - (-1)^{(n+1)} x^{(n+1)} + (-1)^{(n+2)} x^{(n+2)}$

$ = x + (-1)^{(n+2)}x^{(n+2)}$

F端r $x \neq 1 $
$\Rightarrow \sum\limits^{n}_{\nu=1}(-1)^{\nu}x^{\nu} = \frac{x+(-1)^{(n+1)}x^{(n+1)}}{-1-x}$ 

Es folgt $\sum\limits^{\infty}_{\nu=1}(-1)^{\nu}x^{\nu} = \frac{x}{-1-x}$

Also:

$1+2\sum\limits^{\infty}_{\nu=1}(-1)^{\nu}x^{\nu} $

$ = 1+2\frac{x}{-1-x}$

$ = 1 + \frac{-2x}{1+x}$

$ = \frac{1+x-2x}{1+x}$

$ = \frac{1-x}{1+x}$


