\section*{Nr.H6}

\subsection*{i)}

\subsubsection*{Behauptung}

F端r $\sum\limits^{\infty}_{\nu = 1} (x+2)^{\nu} (1+\frac{1}{\nu})^{\nu}$ ist der Konvergenzradius $R = 1$ 

\subsubsection*{Beweis}

$ R = \frac{1}{S}$,
$S = \limsup\limits_{\nu \to \infty} |\sqrt[\nu]{(1 + \frac{1}{\nu})^{\nu}}|
= \limsup\limits_{\nu \to \infty} |1 + \frac{1}{\nu}|
= 1 $,
$R = 1$.

$|x-x_{0}| = |x+2| = 1 = R$ gilt f端r $ x \in \{\-1,-3\}$

\paragraph*{F端r $x = -1$}

$\sum\limits^{\infty}_{\nu = 1}(1+\frac{1}{\nu})^{\nu}$ ist nicht konvergent.


\paragraph*{F端r $x = -3$}

$\sum\limits^{\infty}_{\nu = 1}(-1)^{\nu}(1+\frac{1}{\nu})^{\nu}$

$\limsup\limits_{\nu \to \infty} |\frac{(1+\frac{1}{\nu+1})^{\nu+1}}{(1+\frac{1}{\nu})^{\nu}}|$

$=\limsup\limits_{\nu \to \infty} |(1+\frac{1}{\nu+1})\frac{(1+\frac{1}{\nu+1})^{\nu}}{(1+\frac{1}{\nu})^{\nu}}|$

$=\limsup\limits_{\nu \to \infty} |(1+\frac{1}{\nu+1})(\frac{1+\frac{1}{\nu+1}}{1+\frac{1}{\nu}})^{\nu}|$

$=\limsup\limits_{\nu \to \infty} |(1+\frac{1}{\nu+1})(\frac{v+\frac{v}{\nu+1}}{v+1})^{\nu}|$

$ = 0$ und somit konvergent.


\subsection*{ii) (1-Fach)}

\subsection*{iii) (1-Fach)}
